Refinement form List

theories/Compositional_Structures/Basic_Modules/Plurality_Module_Ref.thy
@@ -50,17 +50,29 @@ lemma nfwcc: "nofail (wc_fold p a)"
  
 
 definition compute_scores :: "'a set \<Rightarrow> 'a Profile_List \<Rightarrow> ('a \<rightharpoonup> nat) nres" 
-  where "compute_scores A p \<equiv> do {
-  (scores) \<leftarrow> FOREACHi (\<lambda>it r. r = (\<lambda> e. Some (win_count (pl_to_pr_\<alpha> p) e)) |` (A - it)) A 
+  where "compute_scores A p \<equiv>
+  FOREACHi (\<lambda>it r. r = (\<lambda> e. Some (win_count (pl_to_pr_\<alpha> p) e)) |` (A - it)) A 
     (\<lambda>x m. do {
       scx \<leftarrow> (wc_fold p x);
       RETURN (m(x\<mapsto>scx))
-  }) (Map.empty);
-  RETURN (scores)
-}"
+  }) (Map.empty)"
 
+definition (*scoremax :: "'a set \<Rightarrow> ('a \<rightharpoonup> nat) \<Rightarrow> nat option nres" 
+  where *)"scoremax A ma \<equiv> do {
+  FOREACH (A)
+  (\<lambda>x m. do {
+      let s = (ma x);
+      if (s > m) then RETURN (s) else RETURN (m)
+  }) (Some 0::nat option) }"
 
-lemma 
+sepref_register scoremax
+
+sepref_definition tryitmap 
+  is "uncurry scoremax" :: "((hs.assn nat_assn)\<^sup>k *\<^sub>a (hm.assn (nat_assn) (nat_assn))\<^sup>k \<rightarrow>\<^sub>a (opt_assn nat_assn))"
+  unfolding scoremax_def[abs_def]
+  apply sepref_dbg_keep
+
+lemma compute_scores_correct:
   fixes pl:: "'a Profile_List" and A:: "'a set"
   assumes "finite A"
   shows "(compute_scores A, ((\<lambda>p. RETURN ((\<lambda>a. Some (win_count p a))|`A))))
@@ -91,7 +103,8 @@ definition (*compute_threshold :: "'a set \<Rightarrow> 'a Profile_List \<Righta
 
 definition plurality_r :: "'a Electoral_Module_Ref" where
   "plurality_r A p \<equiv> do {
-    (scores) \<leftarrow> compute_scores A p; 
+    (scores) \<leftarrow> compute_scores A p;
+    scoremax \<leftarrow> scoremax A scores;
     (e,r,d) \<leftarrow> FOREACH A 
     (\<lambda>x (e,r,d). do {
       ASSERT (x \<in> dom scores);
@@ -112,83 +125,23 @@ sepref_definition plurality_sepref is
    \<rightarrow>\<^sub>a ((hs.assn nat_assn) \<times>\<^sub>a (hs.assn nat_assn) \<times>\<^sub>a (hs.assn nat_assn))"
   unfolding plurality_r_def[abs_def] 
     compute_scores_def[abs_def] wc_fold_def[abs_def] short_circuit_conv
-  apply (rewrite in "FOREACH _ _ \<hole>" hm.fold_custom_empty)
+  apply (rewrite in "FOREACHi _ _ _ \<hole>" hm.fold_custom_empty)
   apply (rewrite in "FOREACH _ _ \<hole>" hs.fold_custom_empty)+
   apply sepref_dbg_keep
   done
 
 lemma datarefplurality:
-  shows "\<forall> A. (plurality_r, (\<lambda> A p. SPEC (\<lambda> elecres. elecres = plurality A p))) \<in> 
-    Id \<rightarrow> (br pl_to_pr_\<alpha> (profile_l A)) \<rightarrow> \<langle>Id\<rangle>nres_rel"
+  shows "finite A \<longrightarrow> ((plurality_r A, (\<lambda> p. SPEC (\<lambda> elecres. elecres = plurality A p))) \<in> 
+    (br pl_to_pr_\<alpha> (profile_l A)) \<rightarrow> \<langle>Id\<rangle>nres_rel)"
   unfolding plurality_r_def FOREACH_def
   compute_scores_def[abs_def]
-  apply (refine_vcg wc_fold_correct)
-  apply (auto simp add: 
-    refine_rel_defs)
+  apply (refine_vcg wc_fold_correct compute_scores_correct)
+  apply (auto simp add:  
+    refine_rel_defs simp del: win_count.simps )
+   apply (metis it_step_insert_iff restrict_map_insert)
+
   
-  done
+  oops
 
-lemma plurality_ref_eq:
-  fixes A :: "'a set" and pa :: "'a Profile_Array"
-  assumes "(profile_a A pa)"
-  shows "plurality_r A pa = plurality A (pa_to_pr pa)"
-  using assms datarefplurality em_onA
-  by blast 
-
-lemma plurality_r_sound:
-  shows "electoral_module_r plurality_r" 
-  unfolding electoral_module_r_def using plurality_sound plurality_ref_eq
-  by (metis electoral_module_def profile_a_rel)
-
-lemma plurality_r_electing2: "\<forall> A pa.
-                              (A \<noteq> {} \<and> finite_profile_a A pa) \<longrightarrow>
-                                elect_r (plurality_r A pa) \<noteq> {}"
-using plurality_electing2 plurality_ref_eq profile_a_rel
-  by metis
-
-theorem plurality_r_electing[simp]: "electing plurality"
-  oops (* Reformulate properties like electing for refined types. Discussion needed*)
-
-(* For further lemmas, Profile definitions have to be transeferred to profile Array
-
-lemma plurality_inv_mono2: "\<forall> A p q a.
-                              (a \<in> elect plurality A p \<and> lifted A p q a) \<longrightarrow>
-                                (elect plurality A q = elect plurality A p \<or>
-                                    elect plurality A q = {a})"*)
-
-(* --------  *)
-  section \<open>Further Refinement: Experiments\<close>
-
-
-type_synonym 'a Electoral_Module_Ref_T = "'a set \<Rightarrow> 'a Profile_Array \<Rightarrow> 'a Result_Ref nres"
-
-definition initmap :: "'a set \<Rightarrow> 'a \<rightharpoonup> nat" where
-  "initmap A = (SOME m. (\<forall>a\<in>A. ((m a) = Some (0::nat))))"
-
-definition "computewcinvar A p \<equiv> \<lambda>(i, wcmap).
-  \<forall>a\<in>A. the (wcmap a) = win_count_imp_code (array_shrink p i) a"
-
-definition computewcforcands :: "'a set \<Rightarrow> 'a Profile_Array \<Rightarrow> ('a \<rightharpoonup> nat) nres" where
-  "computewcforcands A p \<equiv> do {
-    let wcmap = initmap A;               
-    (i, wcmap) \<leftarrow> WHILET (\<lambda>(i, _). i < array_length p) (\<lambda>(i, wcmap). do {
-      ASSERT (i < array_length p);
-      let ballot = (p[[i]]);
-      let wcmap = (if (array_length ballot > 0) then (
-        wcmap ((ballot[[0]]) \<mapsto> (the (wcmap (ballot[[0]]))) + 1)) else wcmap);
-      let i = i + 1;
-     RETURN (i, wcmap)
-    })(0, Map.empty);
-    RETURN wcmap
-  }"
-
-lemma wcmap_correc : assumes "profile_a A p"
-  shows "computewcforcands A p \<le> SPEC (\<lambda> m. \<forall> a \<in> A. (the (m a)) = win_count_imp_code p a)"
-  unfolding computewcforcands_def initmap_def
-  apply (intro WHILET_rule[where I="(computewcinvar A p)" 
-        and R="measure (\<lambda>(i,_). (array_length p) - i)"] refine_vcg)
-  unfolding computewcinvar_def win_count_imp_code_def
-
-  oops (* ambitious goal *)
 
 end
