theories/Compositional_Structures/Basic_Modules/Component_Types/Social_Choice_Types/RefinementList.thy
@@ -1,0 +1,41 @@
+theory RefinementList
+  imports Verified_Voting_Rule_Construction.Preference_Relation
+  Verified_Voting_Rule_Construction.Preference_List
+  Refine_Imperative_HOL.IICF
+
+begin
+
+abbreviation "ballot_rel \<equiv> br (pl_\<alpha>) (well_formed_pl)"
+
+lemma aboveref: 
+  shows "(above_l, above) \<in> ballot_rel \<rightarrow> Id \<rightarrow> \<langle>Id\<rangle>list_set_rel"
+  apply (refine_vcg)
+  apply (auto simp add: refine_rel_defs)
+  unfolding list_set_rel_def
+  by (metis Id_O_R above_l_def aboveeq brI distinct_take list_rel_id_simp well_formed_pl_def)
+  
+lemma rankref: 
+  shows "(rank_l, rank) \<in> ballot_rel \<rightarrow> Id \<rightarrow> nat_rel"
+  apply (refine_vcg rankeq)
+  apply (auto simp only: refine_rel_defs)
+  using rankeq
+    by metis
+
+lemma is_less_preferred_than_ref:
+  shows "(is_less_preferred_than_l, is_less_preferred_than) 
+    \<in> Id \<rightarrow> ballot_rel \<rightarrow> Id \<rightarrow> bool_rel"
+  apply (refine_vcg rankeq)
+  by (auto simp only: refine_rel_defs less_preffered_l_rel_eq)
+
+lemma limitref:
+  shows "(limit_l, limit) \<in> \<langle>Id\<rangle>set_rel \<rightarrow> ballot_rel \<rightarrow> ballot_rel"
+  apply (refine_vcg rankeq)
+  apply (auto simp add: refine_rel_defs)
+  unfolding well_formed_pl_def pl_\<alpha>_def
+  apply auto
+  apply (simp_all add: member_def)
+   apply clarsimp_all
+  oops
+   
+
+end
